Lemma/Int/LeMulS/of/Ge/Le_0.lean
@@ -2,10 +2,17 @@ import Lemma.Int.GeMulS.of.Ge.Ge_0
 import Lemma.Int.GeNeg_0.of.Le_0
 import Lemma.Int.Mul_Neg.eq.NegMul
 import Lemma.Int.Le.of.GeNegS
+import sympy.Basic'
 open Int
 
-
-@[main]
+/--
+using comm 2 instead of comm 1 since conditions of the lemma is arranged according to the constructor of multiplication
+| attributes | lemma |
+| :---: | :---: |
+| main | Int.LeMulS.of.Ge.Le_0 |
+| comm 2 | Int.GeMulS.of.Le.Le_0 |
+-/
+@[main, comm 2]
 private lemma main
   [Ring α] [LinearOrder α] [IsStrictOrderedRing α]
   {x a b : α}
