Lemma/Int/LeMulS/of/Ge/Lt_0.lean
@@ -1,9 +1,16 @@
 import Lemma.Int.LeMulS.of.Ge.Le_0
 import Lemma.Nat.Le.of.Lt
+import sympy.Basic'
 open Nat Int
 
-
-@[main]
+/--
+using comm2 for similar reason of Int.LeMulS.of.Ge.Le_0
+| attributes | lemma |
+| :---: | :---: |
+| main | Int.LeMulS.of.Ge.Lt_0 |
+| comm 2 | Int.GeMulS.of.Le.Lt_0 |
+-/
+@[main, comm 2]
 private lemma main
   [Ring α] [LinearOrder α] [IsStrictOrderedRing α]
   {x a b : α}
