Lemma/Int/LeSubS/is/Le.lean
@@ -1,7 +1,7 @@
 import sympy.Basic
 
 
-@[main, comm, mp, mpr]
+@[main, comm, mp, mpr, mp.comm, mpr.comm, comm.is]
 private lemma main
   [AddGroup α]
   [LE α]
