Lemma/List/LengthSlicedIndices'/eq/CeilDivSub/of/Gt_0/Le/Gt/Sub/le/Mul.lean
@@ -14,7 +14,7 @@ import Lemma.Nat.Gt.of.GtSub
 import Lemma.Rat.DivSub.eq.SubDivS
 import Lemma.Rat.Div.eq.One.of.Gt_0
 import Lemma.Rat.CeilSub_1.eq.SubCeil_1
-import Lemma.Nat.GeAdd.of.Ge_Sub
+import Lemma.Nat.LeSub.is.Le_Add
 import Lemma.Nat.CoeAdd.eq.AddCoeS
 open Nat Int Rat
 
