Lemma/List/SliceTake/eq/Slice/of/Ge.lean
@@ -8,7 +8,7 @@ import Lemma.Bool.NotAnd.is.OrNotS
 import Lemma.Nat.Ge.of.Gt.Ge
 import Lemma.List.EqTake.of.Ge_Length
 import Lemma.List.TakeTake.eq.Take.of.Ge
-import Lemma.Nat.GeSubS.of.Ge
+import Lemma.Nat.LeSubS.of.Le
 import Lemma.List.DropTake.eq.TakeDrop
 open List Bool Nat
 
