Lemma/Nat/LeSubS/of/Le.lean
@@ -1,7 +1,7 @@
 import sympy.Basic
 
 
-@[main]
+@[main, comm 1]
 private lemma main
   {x y : ℕ}
 -- given
