Lemma/Rat/LeToNatCeil_1/of/Ge_Sub.lean
@@ -1,4 +1,4 @@
-import Lemma.Nat.GeAdd.of.Ge_Sub
+import Lemma.Nat.LeSub.is.Le_Add
 import Lemma.Rat.LeToNatCeil_1.of.Le_Add
 open Rat Nat
 
